RISC-V: reworked register file, x0 is no longer an actual register, use of abstract pred (magic wand emulation) for working with gprs, added x3 (no proofs needed modifications to introduce this register)

case_study/RiscvPmp/Contracts.v
@@ -55,6 +55,9 @@ Inductive PurePredicate : Set :=
 Inductive Predicate : Set :=
 | pmp_entries
 | ptsreg
+| gprs
+| gprs_without
+| is_reg
 .
 
 Section TransparentObligations.
@@ -84,15 +87,21 @@ Module Export RiscvPmpAssertionKit <: (AssertionKit RiscvPmpTermKit RiscvPmpProg
   Definition 𝑯 := Predicate.
   Definition 𝑯_Ty (p : 𝑯) : Ctx Ty :=
     match p with
-    | pmp_entries => [ty_list (ty_prod ty_pmpcfg_ent ty_xlenbits)]
-    | ptsreg      => [ty_regidx, ty_xlenbits]
+    | pmp_entries  => [ty_list (ty_prod ty_pmpcfg_ent ty_xlenbits)]
+    | ptsreg       => [ty_regno, ty_xlenbits]
+    | gprs         => ctx.nil
+    | gprs_without => [ty_regno]
+    | is_reg       => [ty_regno]
     end.
 
   Instance 𝑯_is_dup : IsDuplicable Predicate := {
     is_duplicable p :=
       match p with
-      | pmp_entries => false
-      | ptsreg      => false
+      | pmp_entries  => false
+      | ptsreg       => false
+      | gprs         => false
+      | gprs_without => false
+      | is_reg       => true
       end
     }.
   Instance 𝑯_eq_dec : EqDec 𝑯 := Predicate_eqdec.
@@ -106,9 +115,19 @@ Module RiscvPmpSymbolicContractKit <: (SymbolicContractKit RiscvPmpTermKit
                                   RiscvPmpAssertionKit.
 
   Local Notation "r '↦' val" := (asn_chunk (chunk_ptsreg r val)) (at level 100).
-  Local Notation "r '↦r' val" := (asn_chunk (chunk_user ptsreg (env.nil ► (ty_regidx ↦ r) ► (ty_xlenbits ↦ val)))) (at level 100).
+  Local Notation "r '↦r' val" := (asn_chunk (chunk_user ptsreg (env.nil ► (ty_regno ↦ r) ► (ty_xlenbits ↦ val)))) (at level 100).
   Local Notation "p '∗' q" := (asn_sep p q) (at level 150).
   Local Notation asn_pmp_entries l := (asn_chunk (chunk_user pmp_entries (env.nil ► (ty_list (ty_prod ty_pmpcfg_ent ty_xlenbits) ↦ l)))).
+  Local Notation asn_gprs := (asn_chunk (chunk_user gprs env.nil)).
+  Local Notation asn_gprs_without r := (asn_chunk (chunk_user gprs_without (env.nil ► (ty_regno ↦ r)))).
+  Local Notation asn_is_reg r := (asn_chunk (chunk_user is_reg (env.nil ► (ty_regno ↦ r)))).
+
+  Definition term_eqb {Σ} (e1 e2 : Term Σ ty_int) : Term Σ ty_bool :=
+    term_binop binop_eq e1 e2.
+
+  Local Notation "e1 '=?' e2" := (term_eqb e1 e2).
+
+  Definition z_term {Σ} : Z -> Term Σ ty_int := term_lit ty_int.
 
   Definition sep_contract_logvars (Δ : PCtx) (Σ : LCtx) : LCtx :=
     ctx.map (fun '(x::σ) => x::σ) Δ ▻▻ Σ.
@@ -138,20 +157,14 @@ Module RiscvPmpSymbolicContractKit <: (SymbolicContractKit RiscvPmpTermKit
         @asn_exists Σ Γ (asn_exist x τ asn)
     end.
 
-  Definition regidx_to_reg (r : RegIdx) : Reg ty_xlenbits :=
-    match r with
-    | X0 => x0
-    | X1 => x1
-    | X2 => x2
-    end.
-
-  Definition asn_and_regs {Σ} (f : RegIdx -> Assertion Σ) : Assertion Σ :=
-    f X0 ∗ f X1 ∗ f X2.
-
-  (* ∀ r : regidx, ∃ w : xlenbits, r ↦r w *)
-  Definition asn_regs_ptsto {Σ} : Assertion Σ :=
-    asn_and_regs
-      (fun r => asn_exist "w" ty_xlenbits (term_lit ty_regidx r ↦r term_var "w")).
+  Definition asn_with_reg {Σ} (r : Term Σ ty_int) (asn : Reg ty_xlenbits -> Assertion Σ) (asn_default : Assertion Σ) : Assertion Σ :=
+    asn_if (r =? z_term 1)
+           (asn x1)
+           (asn_if (r =? z_term 2)
+                   (asn x2)
+                   (asn_if (r =? z_term 3)
+                           (asn x3)
+                           asn_default)).
 
   (* TODO: abstract away the concrete type, look into unions for that *)
   (* TODO: length of list should be 16, no duplicates *)
@@ -184,11 +197,11 @@ Module RiscvPmpSymbolicContractKit <: (SymbolicContractKit RiscvPmpTermKit
          pc ↦ (term_var "i") ∗
          asn_pmp_entries (term_var "entries") ∗
          asn_exist v ty_xlenbits (nextpc ↦ term_var v) ∗
-         asn_regs_ptsto;
+         asn_gprs;
        sep_contract_result          := "result_mach_inv";
        sep_contract_postcondition   :=
          asn_pmp_entries (term_var "entries") ∗
-         asn_regs_ptsto ∗
+         asn_gprs ∗
          mtvec ↦ (term_var "h") ∗
          asn_exist v ty_xlenbits (nextpc ↦ term_var v) ∗
          asn_or (cur_privilege ↦ (term_var "m") ∗ pc ↦ (term_var "i"))
@@ -277,30 +290,21 @@ Module RiscvPmpSymbolicContractKit <: (SymbolicContractKit RiscvPmpTermKit
     |}.
 
   Definition sep_contract_rX : SepContractFun rX :=
-    {| sep_contract_logic_variables := [rs ∶ ty_regidx, v ∶ ty_xlenbits];
+    {| sep_contract_logic_variables := [rs ∶ ty_regno];
        sep_contract_localstore      := [term_var rs]%arg;
-       sep_contract_precondition    := term_var rs ↦r term_var v;
+       sep_contract_precondition    := asn_gprs;
        sep_contract_result          := "result_rX";
-       sep_contract_postcondition   :=
-         asn_eq (term_var "result_rX") (term_var v)
-         ∗ term_var rs ↦r term_var v
+       sep_contract_postcondition   := asn_gprs;
     |}.
 
   Definition sep_contract_wX : SepContractFun wX :=
-    {| sep_contract_logic_variables := [rs ∶ ty_regidx, v ∶ ty_xlenbits, "v__old" :: ty_xlenbits];
+    {| sep_contract_logic_variables := [rs ∶ ty_regno, v ∶ ty_xlenbits];
        sep_contract_localstore      := [term_var rs, term_var v]%arg;
-       sep_contract_precondition    := term_var rs ↦r term_var "v__old";
+       sep_contract_precondition    := asn_gprs;
        sep_contract_result          := "result_wX";
        sep_contract_postcondition   :=
          asn_eq (term_var "result_wX") (term_lit ty_unit tt)
-         ∗ asn_match_enum
-             regidx (term_var rs)
-             (* TODO: This should only binary branching. *)
-             (fun k => match k with
-                       | X0 => asn_eq (term_var "v__old") (term_lit ty_xlenbits 0) ∗
-                               term_var rs ↦r term_lit ty_xlenbits 0
-                       | _  => term_var rs ↦r term_var v
-                       end);
+         ∗ asn_gprs;
     |}.
 
   Definition sep_contract_abs : SepContractFun abs :=
@@ -335,30 +339,50 @@ Module RiscvPmpSymbolicContractKit <: (SymbolicContractKit RiscvPmpTermKit
        sep_contract_postcondition   := asn_true;
     |}.
 
-  Definition lemma_open_ptsreg : SepLemma open_ptsreg :=
-    {| lemma_logic_variables := [ rs ∶ ty_regidx, w ∶ ty_xlenbits];
-       lemma_patterns        := [term_var rs]%arg;
-       lemma_precondition    := term_var rs ↦r term_var w;
+  Definition lemma_extract_ptsreg : SepLemma extract_ptsreg :=
+    {| lemma_logic_variables := [rs ∶ ty_regno];
+       lemma_patterns        := [term_var rs];
+       lemma_precondition    := asn_gprs ∗ asn_is_reg (term_var rs);
        lemma_postcondition   :=
-         asn_match_enum
-           regidx (term_var rs)
-           (fun k => match k with
-                     | X0 => x0 ↦ term_var w ∗ asn_eq (term_var w) (term_lit ty_xlenbits 0)
-                     | X1 => x1 ↦ term_var w
-                     | X2 => x2 ↦ term_var w
-                     end)
+             asn_exist w ty_xlenbits (term_var rs ↦r term_var w)
+             ∗ asn_gprs_without (term_var rs);
     |}.
 
-  Definition lemma_close_ptsreg (r : RegIdx) : SepLemma (close_ptsreg r) :=
-    {| lemma_logic_variables := [w ∶ ty_xlenbits];
-       lemma_patterns        := env.nil;
-       lemma_precondition    := match r with
-                                | X0 => x0 ↦ term_var w ∗
-                                        asn_eq (term_var w) (term_lit ty_xlenbits 0)
-                                | X1 => x1 ↦ term_var w
-                                | X2 => x2 ↦ term_var w
-                                end;
-       lemma_postcondition   := term_enum regidx r ↦r term_var w;
+  Definition lemma_return_ptsreg : SepLemma return_ptsreg :=
+    {| lemma_logic_variables := [rs ∶ ty_regno];
+       lemma_patterns        := [term_var rs];
+       lemma_precondition    :=
+             asn_is_reg (term_var rs) ∗
+             asn_exist w ty_xlenbits (term_var rs ↦r term_var w) ∗
+             asn_gprs_without (term_var rs);
+       lemma_postcondition   := asn_gprs;
+    |}.
+
+  Definition lemma_open_ptsreg : SepLemma open_ptsreg :=
+    {| lemma_logic_variables := [rs ∶ ty_regno, w ∶ ty_xlenbits];
+       lemma_patterns        := [term_var rs];
+       lemma_precondition    := term_var rs ↦r term_var w;
+       lemma_postcondition   := asn_with_reg (term_var rs)
+                                             (fun r => r ↦ term_var w)
+                                             asn_false;
+    |}.
+
+  Definition lemma_close_ptsreg : SepLemma close_ptsreg :=
+    {| lemma_logic_variables := [rs ∶ ty_regno, w ∶ ty_xlenbits];
+       lemma_patterns        := [term_var rs];
+       lemma_precondition    := asn_with_reg (term_var rs)
+                                             (fun r => r ↦ term_var w)
+                                             asn_false;
+       lemma_postcondition   := term_var rs ↦r term_var w
+    |}.
+
+  Definition lemma_valid_reg : SepLemma valid_reg :=
+    {| lemma_logic_variables := [rs ∶ ty_regno];
+       lemma_patterns        := [term_var rs];
+       lemma_precondition    := asn_with_reg (term_var rs)
+                                             (fun r => asn_true)
+                                             asn_false;
+       lemma_postcondition   := asn_is_reg (term_var rs);
     |}.
 
   End Contracts.
@@ -396,8 +420,11 @@ Module RiscvPmpSymbolicContractKit <: (SymbolicContractKit RiscvPmpTermKit
   Definition LEnv : LemmaEnv :=
     fun Δ l =>
       match l with
+      | extract_ptsreg => lemma_extract_ptsreg
+      | return_ptsreg  => lemma_return_ptsreg
       | open_ptsreg    => lemma_open_ptsreg
-      | close_ptsreg r => lemma_close_ptsreg r
+      | close_ptsreg   => lemma_close_ptsreg
+      | valid_reg      => lemma_valid_reg
       end.
 
   Lemma linted_cenvex :
@@ -548,7 +575,7 @@ Module BlockVerification.
     (chunk_user
        ptsreg
        (env.nil
-          ► (ty_regidx ↦ term_lit ty_regidx r)
+          ► (ty_regno ↦ term_lit ty_regno r)
           ► (ty_xlenbits ↦ val)))
       (at level 100).
   Notation "ω ∣ x <- ma ;; mb" :=
@@ -570,12 +597,8 @@ Module BlockVerification.
     fun _ u0 =>
       ω01 ∣ v1 <- @angelic ty_xlenbits _ ;;
       ω12 ∣ _  <- consume_chunk (r ↦r v1) ;;
-      if eq_dec r X0
-      then let v2 := persist__term v1 ω12 in
-           _ ∣ _ <- assume (formula_eq v2 (term_lit ty_xlenbits 0)) ;;
-           produce_chunk (r ↦r term_lit ty_xlenbits 0)
-      else let u2 := persist__term u0 (acc_trans ω01 ω12) in
-           produce_chunk (r ↦r u2).
+      let u2 := persist__term u0 (acc_trans ω01 ω12) in
+      produce_chunk (r ↦r u2).
 
   Definition exec_rtype (rs2 rs1 rd : RegIdx) (op : ROP) : ⊢ M Unit :=
     fun _ =>
@@ -639,25 +662,25 @@ Module BlockVerification.
          (chunk_user
             ptsreg
             (env.nil
-               ► (ty_regidx ↦ term_lit ty_regidx r)
+               ► (ty_regno ↦ term_lit ty_regno r)
                ► (ty_xlenbits ↦ val))))
          (at level 100).
 
     Example block1 : list AST :=
-      [ ADD X1 X1 X2;
-        SUB X2 X1 X2;
-        SUB X1 X1 X2
+      [ ADD 1 1 2;
+        SUB 2 1 2;
+        SUB 1 1 2
       ].
 
     Let Σ1 : LCtx := ["x" :: ty_xlenbits, "y" :: ty_xlenbits].
 
     Example pre1 : Assertion Σ1 :=
-      X1 ↦r term_var "x" ∗
-      X2 ↦r term_var "y".
+      1 ↦r term_var "x" ∗
+      2 ↦r term_var "y".
 
     Example post1 : Assertion Σ1 :=
-      X1 ↦r term_var "y" ∗
-      X2 ↦r term_var "x".
+      1 ↦r term_var "y" ∗
+      2 ↦r term_var "x".
 
     Example VC1 : 𝕊 Σ1 := VC pre1 block1 post1.
 
