case_study/RiscvPmp/Model.v
@@ -99,21 +99,36 @@ Module RiscvPmpModel.
 
       Definition interp_ptsreg `{sailRegG Σ} (r: RegIdx) (v : Z) : iProp Σ :=
         match r with
-        | X0 => reg_pointsTo x0 v ∗ ⌜v = 0%Z⌝
-        | X1 => reg_pointsTo x1 v
-        | X2 => reg_pointsTo x2 v
+        | 1%Z => reg_pointsTo x1 v
+        | 2%Z => reg_pointsTo x2 v
+        | 3%Z => reg_pointsTo x3 v
+        | _   => False
         end.
+
+      Definition reg_file : gset RegIdx := list_to_set (seqZ 1 3).
+
+      Definition interp_gprs `{sailRegG Σ} : iProp Σ :=
+        [∗ set] r ∈ reg_file, (∃ v, interp_ptsreg r v)%I.
+
+      Definition interp_gprs_without `{sailRegG Σ} (x : RegIdx) : iProp Σ :=
+        [∗ set] r ∈ reg_file ∖ {[ x ]}, (∃ v, interp_ptsreg r v)%I.
+
+      Definition interp_is_reg `{sailRegG Σ} (r : RegIdx) : iProp Σ :=
+        ⌜r ∈ reg_file⌝.
 
       Definition luser_inst `{sailRegG Σ} `{invG Σ} (p : Predicate) (ts : Env Lit (RiscvPmpAssertionKit.𝑯_Ty p)) (mG : memG Σ) : iProp Σ :=
         (match p return Env Lit (RiscvPmpAssertionKit.𝑯_Ty p) -> iProp Σ with
-         | pmp_entries => fun ts => let entries_lst := env.head ts in
+         | pmp_entries  => fun ts => let entries_lst := env.head ts in
                                     match entries_lst with
                                     | (cfg0, addr0) :: [] =>
                                       (reg_pointsTo pmp0cfg cfg0 ∗
                                               reg_pointsTo pmpaddr0 addr0)%I
                                     | _ => False%I
                                     end
-         | ptsreg => fun ts => interp_ptsreg (env.head (env.tail ts)) (env.head ts)
+         | ptsreg       => fun ts => interp_ptsreg (env.head (env.tail ts)) (env.head ts)
+         | gprs         => fun _  => interp_gprs
+         | gprs_without => fun ts => interp_gprs_without (env.head ts)
+         | is_reg       => fun ts => interp_is_reg (env.head ts)
          end) ts.
 
     Definition lduplicate_inst `{sailRegG Σ} `{invG Σ} (p : Predicate) (ts : Env Lit (RiscvPmpAssertionKit.𝑯_Ty p)) :
@@ -142,27 +157,64 @@ Module RiscvPmpModel.
   Section Lemmas.
     Context `{sg : sailG Σ}.
 
+    Lemma valid_reg_sound :
+      ValidLemma RiscvPmpSymbolicContractKit.lemma_valid_reg.
+    Proof.
+      intros ι; destruct_syminstance ι; cbn.
+      unfold RiscvPmpIrisHeapKit.interp_is_reg, RiscvPmpIrisHeapKit.reg_file.
+      rewrite elem_of_list_to_set.
+      iFrame; destruct rs eqn:Ers; cbn;
+        try (iIntros "%H"; destruct H as [H _]; inversion H).
+      repeat (destruct p;
+              try (iIntros "%H"; destruct H as [H _]; inversion H);
+              try (iPureIntro; apply elem_of_seqZ; lia)).
+    Qed.
+
+    Lemma extract_ptsreg_sound :
+      ValidLemma RiscvPmpSymbolicContractKit.lemma_extract_ptsreg.
+    Proof.
+      intros ι; destruct_syminstance ι; cbn.
+      unfold RiscvPmpIrisHeapKit.interp_gprs, RiscvPmpIrisHeapKit.interp_gprs_without,
+        RiscvPmpIrisHeapKit.interp_is_reg.
+      iFrame; iIntros "[Hgprs %Hin]".
+      rewrite big_sepS_delete; try apply Hin.
+      iFrame; iIntros; iAccu.
+    Qed.
+
+    Lemma return_ptsreg_sound :
+      ValidLemma RiscvPmpSymbolicContractKit.lemma_return_ptsreg.
+    Proof.
+      intros ι; destruct_syminstance ι; cbn.
+      unfold RiscvPmpIrisHeapKit.interp_gprs, RiscvPmpIrisHeapKit.interp_is_reg.
+      iFrame; iIntros "[[%Hin Hrs] Hrest]".
+      rewrite big_sepS_delete; try apply Hin.
+      unfold RiscvPmpIrisHeapKit.interp_gprs_without; iAccu.
+    Qed.
+
     Lemma open_ptsreg_sound :
       ValidLemma RiscvPmpSymbolicContractKit.lemma_open_ptsreg.
     Proof.
       intros ι; destruct_syminstance ι; cbn.
-      destruct rs; auto. cbn.
-      iIntros "[H1 H2]"; auto.
+      unfold RiscvPmpIrisHeapKit.interp_ptsreg.
+      destruct rs; auto.
+      repeat (destruct p; auto).
     Qed.
 
-    Lemma close_ptsreg_sound {R} :
-      ValidLemma (RiscvPmpSymbolicContractKit.lemma_close_ptsreg R).
+    Lemma close_ptsreg_sound :
+      ValidLemma RiscvPmpSymbolicContractKit.lemma_close_ptsreg.
     Proof.
       intros ι; destruct_syminstance ι; cbn.
-      unfold RiscvPmpSymbolicContractKit.regidx_to_reg; destruct R; auto.
-      cbn.
-      iIntros "[H1 [H21 H22]]"; auto.
+      destruct rs; cbn; iFrame; try (iIntros "[%H _]"; inversion H).
+      repeat (destruct p;
+              try (iIntros "[%H _]"; inversion H);
+              try (iIntros; iAccu)).
     Qed.
   End Lemmas.
 
   Lemma lemSem `{sg : sailG Σ} : LemmaSem (Σ := Σ).
   Proof.
     intros Δ [];
-      eauto using open_ptsreg_sound, close_ptsreg_sound.
+      eauto using valid_reg_sound, extract_ptsreg_sound, return_ptsreg_sound,
+                  open_ptsreg_sound, close_ptsreg_sound.
   Qed.
 End RiscvPmpModel.
